Add `keccak_map` to `preserved` relation

Clear/EVMState.lean
@@ -167,24 +167,29 @@ abbrev EVM := EVMState
 def preserved : EVMState → EVMState → Prop :=
   (Eq on EVMState.account_map) ∩
   (Eq on EVMState.hash_collision) ∩
-  (Eq on EVMState.execution_env)
+  (Eq on EVMState.execution_env) ∩
+  (Eq on EVMState.keccak_map)
 
 lemma preserved_def {e₀ e₁ : EVM} : preserved e₀ e₁ =
   (e₀.account_map   = e₁.account_map ∧
   e₀.hash_collision = e₁.hash_collision ∧
-  e₀.execution_env  = e₁.execution_env) := by
+  e₀.execution_env = e₁.execution_env ∧
+  e₀.keccak_map = e₁.keccak_map)  := by
   unfold preserved
   dsimp [(· ∩ ·)]
   simp [Function.onFun, and_assoc]
 
 def preserves_account_map {evm evm' : EVMState} (h : preserved evm evm') :
-  evm.account_map = evm'.account_map := h.1.1
+  evm.account_map = evm'.account_map := h.1.1.1
 
 def preserves_collision {evm evm' : EVMState} (h : preserved evm evm') :
-  evm.hash_collision = evm'.hash_collision := h.1.2
+  evm.hash_collision = evm'.hash_collision := h.1.1.2
 
 def preserves_execution_env {evm evm' : EVMState} (h : preserved evm evm') :
-  evm.execution_env = evm'.execution_env := h.2
+  evm.execution_env = evm'.execution_env := h.1.2
+
+def preserves_keccak_map {evm evm' : EVMState} (h : preserved evm evm') :
+  evm.keccak_map = evm'.keccak_map := h.2
 
 @[simp]
 lemma preserved_rfl {e : EVM} : preserved e e := by
@@ -199,7 +204,8 @@ lemma preserved_trans {e₀ e₁ e₂ : EVM} :
   have acc := Eq.trans (preserves_account_map h₀) (preserves_account_map h₁)
   have col := Eq.trans (preserves_collision h₀) (preserves_collision h₁)
   have env := Eq.trans (preserves_execution_env h₀) (preserves_execution_env h₁)
-  constructor; swap; constructor
+  have kec := Eq.trans (preserves_keccak_map h₀) (preserves_keccak_map h₁)
+  constructor; swap; constructor; swap; constructor
   all_goals assumption
 
 -- functions for querying balance
